commit

AP/Inference/Basic.lean
@@ -7,17 +7,30 @@ inductive Expr where
 | not : Expr → Expr
 | imp : Expr → Expr → Expr
 
-inductive Proof : Expr → Prop where
-| ax₁ : ∀ (P Q : Expr), Proof # .imp P # .imp Q P
-| ax₂ : ∀ (P Q R : Expr), Proof # .imp
+inductive Proof' : Expr → Type where
+| ax₁ : ∀ (P Q : Expr), Proof' # .imp P # .imp Q P
+| ax₂ : ∀ (P Q R : Expr), Proof' # .imp
   (.imp P # .imp Q R) # .imp (.imp P Q) # .imp P R
-| ax₃ : ∀ (P Q : Expr), Proof # .imp
+| ax₃ : ∀ (P Q : Expr), Proof' # .imp
   (.imp (.not P) (.not Q)) # .imp Q P
-| mp : ∀ {P Q}, Proof (.imp P Q) → Proof P → Proof Q
+| mp : ∀ {P Q}, Proof' (.imp P Q) → Proof' P → Proof' Q
 
-open Proof
+inductive Proof (e : Expr) : Prop where
+| mk : Proof' e → Proof e
 
 -----
+
+noncomputable
+def Proof.p {e} (h : Proof e) : Proof' e := by
+  apply Nonempty.some; cases h; nm h; use h
+
+@[match_pattern] def ax₁ P Q := Proof.mk # Proof'.ax₁ P Q
+@[match_pattern] def ax₂ P Q R := Proof.mk # Proof'.ax₂ P Q R
+@[match_pattern] def ax₃ P Q := Proof.mk # Proof'.ax₃ P Q
+
+@[match_pattern]
+def mp {P Q : Expr} (h₁ : Proof # .imp P Q) (h₂ : Proof _) :=
+  Proof.mk # Proof'.mp h₁.p h₂.p
 
 theorem mp' {P Q} (h₁ : Proof P) (h₂ : Proof # .imp P Q) : Proof Q :=
   mp h₂ h₁
@@ -27,3 +40,110 @@ theorem imp_refl : Proof # .imp (.var 0) (.var 0) := by
   apply mp' # ax₁ P P
   apply mp' # ax₁ P (.imp P P)
   exact ax₂ P (.imp P P) P
+
+@[simp]
+def Expr.subst (e : Expr) (i : ℕ) (e' : Expr) : Expr :=
+  match e with
+  | .var j => if j = i then e' else e
+  | .not e => .not # e.subst i e'
+  | .imp a b => .imp (a.subst i e') (b.subst i e')
+
+@[simp]
+def proof_subst_of' {e e' i} (p : Proof' e) : Proof' # e.subst i e' :=
+  match hp : p with
+  | .ax₁ P Q => by nm h₁; subst h₁; simp at hp ⊢; subst hp; apply Proof'.ax₁
+  | .ax₂ P Q R => by nm h₁; subst h₁; simp at hp ⊢; subst hp; apply Proof'.ax₂
+  | .ax₃ P Q => by nm h₁; subst h₁; simp at hp ⊢; subst hp; apply Proof'.ax₃
+  | .mp p₁ p₂ => by
+    nm a b h₁; subst h₁; simp at hp; subst hp; have p₁' := @proof_subst_of' _ e' i p₁
+    have p₂' := @proof_subst_of' _ e' i p₂; simp at p₁'; exact Proof'.mp p₁' p₂'
+termination_by sizeOf p
+decreasing_by all_goals
+  nm a b p' h₁ h₂; subst h₁; simp at h₂ hp; subst h₂; rw [hp]; simp; try linarith
+
+theorem proof_subst_of {e e' i} (h : Proof e) : Proof # e.subst i e' :=
+  ⟨proof_subst_of' h.p⟩
+
+@[simp]
+def Proof'.nodes {e} (p : Proof' e) : Set # Σ e, Proof' e :=
+  match h₁ : p with
+  | .ax₁ _ _ => {⟨e, p⟩}
+  | .ax₂ _ _ _ => {⟨e, p⟩}
+  | .ax₃ _ _ => {⟨e, p⟩}
+  | .mp p₁ p₂ => by nm e p₃ h₂; subst h₂; exact insert ⟨e, p⟩ # p₁.nodes ∪ p₂.nodes
+termination_by sizeOf p
+decreasing_by all_goals
+  nm a b p' h₂; subst h₂; simp at h₁ hp; subst hp; rw [h₁]; simp; try linarith
+
+@[simp]
+theorem mem_nodes_self {e} {p : Proof' e} : ⟨e, p⟩ ∈ p.nodes := by
+  cases p <;> simp
+
+-- #check 0 #exit
+
+theorem sizeOf_lt_of_mem_nodes {e e'} {p : Proof' e} {p' : Proof' e'}
+(h₁ : ⟨e', p'⟩ ∈ p.nodes) (h₂ : e' ≠ e ∨ ¬(p' ≍ p)) : sizeOf p' < sizeOf p := by
+  fun_induction Proof'.nodes
+  any_goals
+    simp at h₁; rcases h₁ with ⟨rfl, h₁⟩; simp at h₁ h₂; contradiction
+  nm b a p₁ p₂ ih₁ ih₂ h₁; simp
+  rcases h₁ with h₁ | h₁
+  · by_cases h₃ : e' = .imp a b ∧ p' ≍ p₁
+    · rcases h₃ with ⟨rfl, h₃⟩
+      simp at h₃
+      subst h₃
+      linarith
+    rw [not_and_iff_or] at h₃
+    specialize ih₁ p₁ (by simp) h₁ h₃
+    linarith
+  · by_cases h₃ : e' = a ∧ p' ≍ p₂
+    · rcases h₃ with ⟨rfl, h₃⟩
+      simp at h₃
+      subst h₃
+      linarith
+    rw [not_and_iff_or] at h₃
+    specialize ih₂ p₁ (by simp) h₁ h₃
+    linarith
+
+theorem sizeOf_le_of_mem_nodes {e e'} {p : Proof' e} {p' : Proof' e'}
+(h : ⟨e', p'⟩ ∈ p.nodes) : sizeOf p' ≤ sizeOf p := by
+  by_cases h₁ : e' ≠ e ∨ ¬(p' ≍ p)
+  · exact le_of_lt # sizeOf_lt_of_mem_nodes h h₁
+  push_neg at h₁
+  rcases h₁ with ⟨rfl, h₁⟩
+  simp at h₁
+  rw [h₁]
+
+-- theorem mem_nodes_of_imp_var {a i} (p₁ : Proof' a) (p₂ : Proof' # .imp a # .var i) :
+-- ∃ (p : Proof' # .var i), ⟨_, p⟩ ∈ p₂.nodes := by
+--   cases h₁ : p₂
+--   nm b p₃ p₄
+--   subst h₁
+--   simp
+--   sorry
+-- 
+-- -- #check 0 #exit
+-- 
+-- @[simp]
+-- theorem not_proof_var {i} : ¬Proof (.var i) := by
+--   classical
+--   rintro h
+--   replace h : ∃ (n : ℕ) (p : Proof' # .var i), sizeOf p = n
+--   · simp; exact ⟨h.p⟩
+--   replace h : ∃ (p : Proof' # .var i), ∀ (p' : Proof' # .var i), sizeOf p ≤ sizeOf p'
+--   · replace h := Nat.exi_least_of_exi h
+--     rcases h with ⟨n, ⟨p, rfl⟩, h⟩
+--     use p
+--     intro p'
+--     by_contra! h₁
+--     specialize h _ h₁
+--     simp at h
+--   obtain ⟨p, h⟩ := h
+--   cases h₁ : p
+--   nm b p₁ p₂
+--   subst h₁
+--   choose p h₁ using mem_nodes_of_imp_var p₁ p₂
+--   replace h₁ := sizeOf_lt_of_mem_nodes h₁ (by simp)
+--   specialize h p
+--   simp at h
+--   linarith
